Move out more code

ecoop17/dot_storeless_subst_aux.v
@@ -49,99 +49,6 @@ Hint Resolve env_closed_upgrade.
 
 Hint Constructors Forall.
 
-(* Anomaly! *)
-(* Program Lemma index_sigT : forall {X} vs (n : id), n < length vs -> *)
-(*                        {T:X & index (proj1_sig n) vs = Some T}. *)
-
-Program Lemma index_sigT : forall {X} vs (n : id), n < length vs ->
-                       {T:X & index n vs = Some T}.
-Proof.
-  intros; induction vs; simpl in *.
-  - omega.
-  - case_match; beq_nat; subst; eauto.
-Defined.
-
-Definition indexTot {X} (xs : list X) (n : id) (H : n < length xs): X :=
-  projT1 (index_sigT xs n H).
-
-Program Fixpoint vr_subst_all_tot i (env: list vr) (v: vr) (_ : vr_closed i (length env) v) { struct v }: vr :=
-  match v with
-    | VarF x => VarF x
-    | VarB x => indexTot env x _
-    | VObj dms =>
-      let dms' := dms_subst_all_tot i (VarB 0 :: env) dms _ in
-      VObj dms'
-  end
-with subst_all_tot i (env: list vr) (T: ty) (_ : closed i (length env) T){ struct T }: ty :=
-  match T with
-    | TTop        => TTop
-    | TBot        => TBot
-    | TSel v1 l     =>
-      let v1' := vr_subst_all_tot i env v1 _ in
-      TSel v1' l
-    | TFun l T1 T2  =>
-      let T1' := subst_all_tot i env T1 _ in
-      let T2' := subst_all_tot i (VarB 0 :: env) T2 _ in
-      TFun l T1' T2'
-    | TMem l T1 T2  =>
-      let T1' := subst_all_tot i env T1 _ in
-      let T2' := subst_all_tot i env T2 _ in
-      TMem l T1' T2'
-    | TBind T1    =>
-      let T1' := subst_all_tot i (VarB 0 :: env) T1 _ in
-      TBind T1'
-    | TAnd T1 T2  =>
-      let T1' := subst_all_tot i env T1 _ in
-      let T2' := subst_all_tot i env T2 _ in
-      TAnd T1' T2'
-    | TOr T1 T2   =>
-      let T1' := subst_all_tot i env T1 _ in
-      let T2' := subst_all_tot i env T2 _ in
-      TOr T1' T2'
-  end
-with tm_subst_all_tot i (env: list vr) (t: tm) (_ : tm_closed i (length env) t) { struct t }: tm :=
-   match t with
-     | tvar v => let v' := vr_subst_all_tot i env v _ in tvar v'
-     | tapp t1 l t2 =>
-       let t1' := tm_subst_all_tot i env t1 _ in
-       let t2' := tm_subst_all_tot i env t2 _ in
-       tapp t1' l t2'
-   end
-with dm_subst_all_tot i (env: list vr) (d: dm) (_ : dm_closed i (length env) d) { struct d }: dm :=
-   match d with
-     | dfun T1 T2 t2 =>
-       let T1' := subst_all_tot i env T1 _ in
-       let T2' := subst_all_tot i (VarB 0 :: env) T2 _ in
-       let t2' := tm_subst_all_tot i (VarB 0 :: env) t2 _ in
-       dfun T1' T2' t2'
-     | dty T1 =>
-       let T1' := subst_all_tot i env T1 _ in
-       dty T1'
-   end
-with dms_subst_all_tot i (env: list vr) (ds: dms) (_ : dms_closed i (length env) ds) { struct ds }: dms :=
-   match ds with
-     | dnil => dnil
-     | dcons d ds =>
-       let d'  := dm_subst_all_tot i env d _ in
-       let ds' := dms_subst_all_tot i env ds _ in
-       dcons d' ds'
-   end.
-Solve All Obligations with program_simpl; abstract (inverts H; auto).
-
-
-Ltac reduce_indexTot :=
-  try match goal with
-  | H : context [ indexTot ?env ?i _] |- _ => unfold indexTot in *; destruct (index_sigT env i)
-  | |- context [ indexTot ?env ?i _] => unfold indexTot in *; destruct (index_sigT env i)
-  end.
-
-Program Definition ex_type := forall i l v, subst_all_tot i [v] (TSel (VarB 0) l) _ = TSel v l.
-Program Lemma ex: ex_type.
-Proof. red; intros; simpl; reduce_indexTot; simpl in *; congruence. Qed.
-Program Definition ex2_type:= forall i l v0 v1, subst_all_tot i [v1, v0] (TSel (VarB 1) l) _ = TSel v1 l.
-Program Lemma ex2: ex2_type.
-Proof. red; intros; intros; simpl; reduce_indexTot; simpl in *; congruence. Qed.
-
 Lemma index_Forall:
   forall {X} (env : list X) i P, Forall P env -> i < length env ->
                             exists v, index i env = Some v /\ P v.
@@ -159,36 +66,16 @@ Qed.
 (* Can't work because there's no constant head symbol in the conclusion, so auto wouldn't know when to try this out. So we write apply_Forall. *)
 (* Hint Resolve index_Forall'. *)
 
-Lemma indexTot_Forall: forall {X} (env: list X) i (P: X -> Prop) (Henv: Forall P env) (Hlen: i < length env),
-    P (indexTot env i Hlen).
-Proof.
-  unfold indexTot; intros; destruct (index_sigT env i);
-    (* A special case of apply_Forall below *)
-    lets ?: @index_Forall' ___ Henv; eauto.
-Qed.
-
 (* Use "solve" because in subst_all_res_closed_rec this tactic leads the proof
    search down the wrong path whenever it doesn't solve the goal immediately;
    using "solve" is sort of what eauto's proof search and backtracking would do
    anyway: if applying this lemma and searching further doesn't help, backtrack. *)
 Ltac apply_Forall :=
   match goal with
-  | H: Forall ?P ?env |- ?P (indexTot ?env _ _) => try solve [eapply indexTot_Forall; eauto]
   | H: Forall ?P ?env |- ?P _ => try solve [eapply (index_Forall' _ _ _ H); eauto]
   end.
 (* Seems to actually work fine, but this is needed too seldom for now, and can be expensive. *)
 (* Hint Extern 5 => apply_Forall. *)
-
-(* subst_all_closed_upgrade_rec *)
-Lemma subst_all_res_closed_rec:
-  (forall v, forall i k env, Forall (vr_closed i k) env -> forall (Hcl: vr_closed i (length env) v), vr_closed i k (vr_subst_all_tot i env v Hcl)) /\
-  (forall T, forall i k env, Forall (vr_closed i k) env -> forall (Hcl: closed i (length env) T), closed i k (subst_all_tot i env T Hcl)) /\
-  (forall t, forall i k env, Forall (vr_closed i k) env -> forall (Hcl: tm_closed i (length env) t), tm_closed i k (tm_subst_all_tot i env t Hcl)) /\
-  (forall dm, forall i k env, Forall (vr_closed i k) env -> forall (Hcl: dm_closed i (length env) dm), dm_closed i k (dm_subst_all_tot i env dm Hcl)) /\
-  (forall dms, forall i k env, Forall (vr_closed i k) env -> forall (Hcl: dms_closed i (length env) dms), dms_closed i k (dms_subst_all_tot i env dms Hcl)).
-Proof.
-  apply syntax_mutind; intros; simpl in *; inverts_closed; solve [apply_Forall | eauto 11].
-Qed.
 
 Lemma step_closed: forall e v i k, step e v -> tm_closed i k e -> tm_closed i k v.
 Proof.
@@ -269,19 +156,6 @@ with dms_subst_all (env: list vr) (ds: dms) { struct ds }: option dms :=
        ds' <- dms_subst_all env ds;
        ret (dcons d' ds')
    end.
-
-(* (* SearchPattern ((?A -> Prop) -> list ?A -> Prop). *) *)
-(* Lemma subst_all_closed_upgrade_rec_vr: *)
-(*   forall env i, *)
-(*     Forall (vr_closed i 0) env -> *)
-(*     forall j v, *)
-(*       vr_closed i j v -> length env = j -> *)
-(*       exists v', vr_subst_all env v = Some v' /\ *)
-(*             vr_closed i 0 v'. *)
-(* Proof. *)
-(*   intros * HenvCl; induction v; intros * Hcl Hlen; simpl in *; inverse Hcl; *)
-(*   intuition eauto using index_Forall. *)
-(* Abort. *)
 
 Lemma subst_all_success_rec:
   (forall v, forall i env, forall j, vr_closed i j v -> length env = j -> exists v', vr_subst_all env v = Some v') /\
@@ -426,27 +300,6 @@ Qed.
 (*   simpl. *)
 (*   easy. *)
 (* Qed. *)
-
-Lemma closed_irrelevance_rec:
-  (forall i k x (H1 H2: vr_closed i k x), H1 = H2) /\
-  (forall i k T (H1 H2: closed i k T), H1 = H2) /\
-  (forall i k t (H1 H2: tm_closed i k t), H1 = H2) /\
-  (forall i k dm (H1 H2: dm_closed i k dm), H1 = H2) /\
-  (forall i k dms (H1 H2: dms_closed i k dms), H1 = H2).
-Proof.
-  apply closed_mutind; intros; depelim H2; fequal; eauto using le_unique.
-Qed.
-
-Lemma closed_irrelevance: forall T i k (H1 H2: closed i k T), H1 = H2.
-Proof. destruct closed_irrelevance_rec; ev; eauto. Qed.
-Lemma tm_closed_irrelevance: forall i k t (H1 H2: tm_closed i k t), H1 = H2.
-Proof. destruct closed_irrelevance_rec; ev; eauto. Qed.
-Lemma vr_closed_irrelevance: forall i k x (H1 H2: vr_closed i k x), H1 = H2.
-Proof. destruct closed_irrelevance_rec; ev; eauto. Qed.
-Lemma dm_closed_irrelevance: forall i k d (H1 H2: dm_closed i k d), H1 = H2.
-Proof. destruct closed_irrelevance_rec; ev; eauto. Qed.
-Lemma dms_closed_irrelevance: forall i k d (H1 H2: dms_closed i k d), H1 = H2.
-Proof. destruct closed_irrelevance_rec; ev; eauto. Qed.
 
 Lemma steps_closed: forall e v n i k, steps e v n -> tm_closed i k e -> tm_closed i k v.
 Proof. intros * Hst; induction Hst; eauto using step_closed. Qed.
